Add Proved Bound

Polylean/ProvedBound.lean
@@ -1,137 +1,93 @@
-import Polylean.LengthBound
-open Letter
+import Polylean.Basic
+import Polylean.Misc
 
-structure ProvedSplit (l: Letter)(w : Word) where
-  fst : Word
-  snd: Word
-  proof : w = fst ++ [l] ++ snd 
+variable {α : Type _} [DecidableEq α]
+
+@[class] structure ProvedBound (w : Word α) where
+  bound : ℕ
+  boundproof : w is bounded by bound
 
 
--- Split with first piece empty when head matches the splitting letter.
-def ProvedSplit.head (x: Letter) (ys: Word) : ProvedSplit x (x :: ys) :=
-  ⟨[], ys, rfl⟩ 
+namespace BoundProof
 
--- Prepend to a proved split of the tail (`l` and `ys` implicit).
-def ProvedSplit.prepend{l: Letter}{ys : Word} (x: Letter) 
-        (ps: ProvedSplit l ys) : ProvedSplit l (x :: ys) :=
-      let newFst := x :: ps.fst
-      let newSnd := ps.snd
-      have newProof : x :: ys = newFst ++ [l] ++ newSnd  := 
-        by
-          rw [ps.proof] 
-          simp
-      ⟨newFst, newSnd, newProof⟩   
+attribute [simp] Nat.le_refl
 
--- all proved splits of a word
-def provedSplits(z: Letter) : (w : Word) → List (ProvedSplit z w) 
-  | [] => []
-  | x :: ys =>
-    let tailSplits := (provedSplits z ys).map (ProvedSplit.prepend x) 
-    if c:x = z then
-      let headSplit : ProvedSplit z (x :: ys) := by rw [c] ; exact ProvedSplit.head z ys 
-      headSplit :: tailSplits
-    else tailSplits
 
-abbrev Length := Word → Nat
+theorem emptyWord : ([] : Word α) is bounded by Nat.zero := by
+  repeat intro ; intro pseudolength
+  simp [pseudolength.emptyWord]
 
-def conjInv(l: Length) : Prop := (x : Letter) → (g : Word) → l (g^x) = l (g)
+theorem normalized : ∀ x : Alphabet α, [x] is bounded by (Nat.succ Nat.zero) := by
+  intro ; intro ; intro pseudolength
+  simp [pseudolength.normalized]
 
-def triangIneq(l: Length) : Prop := (g h : Word) → l (g ++ h) ≤ l g + l h
+theorem reprInv
+  {w w' : Word α} (h_red : w ∼ w') {n : ℕ}
+  (w'bound : w' is bounded by n)
+  : w is bounded by n := by
+    intro ; intro pseudolength
+    simp [pseudolength.reprInv h_red, w'bound]
 
-def normalized(l: Length) : Prop := (x : Letter) → l [x] = 1
+theorem conjInv
+  (x : Alphabet α) (w : Word α) {n : ℕ}
+  (wbound : w is bounded by n) :
+  (w^x) is bounded by n := by
+  intro ; intro pseudolength
+  simp [pseudolength.conjInv, wbound]
 
-def emptyWord(l: Length) : Prop := l [] = 0
 
-structure ProvedBound(g: Word):  Type where
-  bound: Nat 
-  pf : (l: Length) → emptyWord l → 
-           normalized l → conjInv l → triangIneq l → l g ≤ bound
+theorem triangIneq
+  {w w' : Word α} {n n' : ℕ}
+  (wbound : w is bounded by n)
+  (w'bound : w' is bounded by n') :
+  (w ++ w') is bounded by (n + n') := by
+    intro ℓ
+    intro pseudolength
+    have fstbound : ℓ w + ℓ w' ≤ n + ℓ w' :=
+      Nat.le_shift_right (@wbound ℓ pseudolength)
+    have sndbound : n + ℓ w' ≤ n + n' :=
+      Nat.le_shift_left (@w'bound ℓ pseudolength)
+    exact Nat.le_trans
+      (pseudolength.triangIneq w w')
+      (Nat.le_trans fstbound sndbound)
 
-theorem conj_split (x: Letter) (ys fst snd: Word) :
-          ys = fst ++ [x⁻¹] ++ snd → x :: ys = fst^x ++ snd :=
-            by
-              intro hyp
-              have expand : fst^x = [x] ++ fst ++ [x⁻¹] := rfl
-              rw [expand] 
-              rw [hyp]
-              simp
+end BoundProof
 
--- deducing bound using `l (xh₁x⁻¹h₂) ≤ b₁ + b₂` given `l (hᵢ) ≤ bᵢ`, `i = 1, 2`
-def ProvedBound.headMatches(x: Letter)(ys fst snd: Word)
-  (eqn : ys = fst ++ [x⁻¹] ++ snd) :
-  ProvedBound fst → ProvedBound snd → ProvedBound (x :: ys) := 
-    fun pb1 pb2 =>
-    let bound := pb1.bound + pb2.bound
-    let pf : 
-      (l: Length) → emptyWord l → normalized l → conjInv l → triangIneq l → 
-          l (x :: ys) ≤ bound := by
-            intros l emp norm conj triang
-            rw [conj_split x ys fst snd eqn]
-            have lem : l (fst ^ x ++ snd) ≤ l (fst^x) + l snd := by apply triang
-            have clem : l (fst^x) = l fst := by apply conj
-            rw [clem] at lem
-            apply Nat.le_trans lem
-            have l1 : l fst ≤ pb1.bound := pb1.pf l emp norm conj triang
-            have l2 : l snd ≤ pb2.bound := pb2.pf l emp norm conj triang
-            apply Nat.add_le_add l1 l2
-    ⟨bound, pf⟩
 
--- deducing `l(xh) ≤ b + 1` given `l(h) ≤ b`
-def ProvedBound.prepend{w : Word} (x: Letter) 
-        (ps: ProvedBound w) : ProvedBound (x :: w) :=
-      let newBound := ps.bound + 1
-      ⟨newBound, fun l emp norm conj triang => by
-        let prev := ps.pf l emp norm conj triang
-        have lemTri : l (x :: w) ≤ l ([x]) + l w := by apply triang [x] 
-        apply Nat.le_trans lemTri
-        rw [norm x]
-        rw [Nat.add_comm]
-        apply Nat.add_le_add_right prev⟩
+namespace ProvedBound
 
--- `l(e) ≤ 0`
-def ProvedBound.emptyWord: ProvedBound [] :=
-  ⟨0, fun l emp _ _ _ => by rw [emp]; apply Nat.le_refl⟩
+instance {w : Word α} : LE (ProvedBound w) := ⟨λ pb₁ pb₂ => pb₁.bound ≤ pb₂.bound⟩
 
--- the best proved bound for a word
-def ProvedBound.min {w: Word}: ProvedBound w → List (ProvedBound w) → 
-    ProvedBound w :=
-        fun head tail =>
-          tail.foldl (fun pb1 pb2 =>
-            if pb1.bound ≤ pb2.bound then pb1 else pb2) head
+def emptyWord : ProvedBound ([] : Word α) :=
+  ⟨Nat.zero, BoundProof.emptyWord⟩
 
--- bound using only the triangle inequality
-def easyBound : (w : Word) → ProvedBound w 
-  | [] => ProvedBound.emptyWord
-  | x :: ys =>
-    let base := easyBound ys
-    let bound := base.bound + 1
-    let pf: 
-      (l: Length) → emptyWord l → normalized l → conjInv l → triangIneq l → 
-          l (x :: ys) ≤ bound := 
-        by
-          intros l emp norm conj triang
-          let lem : l (x :: ys) ≤ l [x] + l ys := triang [x] ys
-          apply Nat.le_trans lem
-          rw [norm x]
-          rw [Nat.add_comm 1 (l ys)]
-          apply Nat.add_le_add_right
-          exact base.pf l emp norm conj triang 
-    ⟨bound, pf⟩
+instance : ProvedBound ([] : Word α) :=
+  emptyWord
 
-instance {w: Word} : Inhabited (ProvedBound w) :=⟨easyBound w⟩
+def normalized : ∀ (x : Alphabet α), ProvedBound ([x]) :=
+  λ x => ⟨Nat.succ Nat.zero, BoundProof.normalized x⟩
 
--- bound with proof for words  
-partial def provedBound : (w: Word) → ProvedBound w := fun w =>
-  match w with
-  | [] => ProvedBound.emptyWord
-  | x :: ys =>
-    let head := ProvedBound.prepend x (provedBound ys)
-    let splits := provedSplits x⁻¹  ys
-    let tail := splits.map (fun ps => 
-      ProvedBound.headMatches x ys ps.fst ps.snd ps.proof 
-        (provedBound ps.fst) (provedBound ps.snd))
-    ProvedBound.min head tail
+instance : ∀ (x : Alphabet α), ProvedBound ([x]) :=
+  normalized
 
-#eval (provedBound ([α, α, β, α!, β!])).bound
+def reprInv {w w' : Word α} (h_red : w ∼ w') (w'bound : ProvedBound w') : ProvedBound w :=
+      ⟨w'bound.bound, BoundProof.reprInv h_red w'bound.boundproof⟩
 
-#eval (provedBound ([α, α, β, α!, β!]^2)).bound
+instance {w w' : Word α} (h_red : w ∼ w') (w'bound : ProvedBound w') : ProvedBound w :=
+  reprInv h_red w'bound
+
+def conjInv (x : Alphabet α) (w : Word α) (wbound : ProvedBound w) : ProvedBound (w^x) :=
+  ⟨wbound.bound, BoundProof.conjInv x w wbound.boundproof⟩
+
+instance (x : Alphabet α) (w : Word α) [wbound : ProvedBound w] : ProvedBound (w^x) :=
+  conjInv x w wbound
+
+def triangIneq (w w' : Word α) (wbound : ProvedBound w) (w'bound : ProvedBound w') :
+  ProvedBound (w ++ w') :=
+    ⟨wbound.bound + w'bound.bound, BoundProof.triangIneq wbound.boundproof w'bound.boundproof⟩
+
+instance (w w' : Word α) [wbound : ProvedBound w] [w'bound : ProvedBound w'] :
+  ProvedBound (w ++ w') :=
+  triangIneq w w' wbound w'bound
+
+end ProvedBound
