Polylean/Misc.lean
@@ -1,0 +1,15 @@
+namespace Nat
+
+protected theorem le_shift_left {a b c : Nat} : a ≤ b → c + a ≤ c + b := by
+  intro h
+  induction c with
+  | zero => simp [h]
+  | succ _ ih => simp [Nat.succ_add, Nat.succ_le_succ ih]
+
+protected theorem le_shift_right {a b c : Nat} : a ≤ b → a + c ≤ b + c := by
+  intro h
+  induction c with
+    | zero => simp [h]
+    | succ _ ih => simp [Nat.add_succ, Nat.succ_le_succ ih]
+
+end Nat
